theories/XChecking.v
@@ -5,7 +5,7 @@ From Equations Require Import Equations DepElimDec.
 From Template Require Import utils Ast Typing Checker.
 From Translation Require Import util Quotes Sorts SAst SLiftSubst SCommon
      ITyping ITypingInversions ITypingLemmata ITypingAdmissible XTyping
-     FundamentalLemma Translation FinalTranslation FullQuote ExampleQuotes
+     FundamentalLemma Translation FinalTranslation FullQuote
      IChecking XTypingLemmata XInversions.
 
 (* For efficiency reasons we use type in type for examples. *)
