theories/plugin_demo.v
@@ -1,0 +1,60 @@
+(* This file illustrates the use of the plugin from ett to itt on examples. *)
+
+From Translation Require Import complex_demo.
+
+(* Definition AA := Type. *)
+(* Run TemplateProgram (Θ <- TranslateConstant ε "AA" ;; tmPrint Θ). *)
+(* Run TemplateProgram (TranslateConstant ε "Init.Nat.add"). *)
+
+(* Run TemplateProgram (Θ <- TranslateConstant ε "nat" ;; Θ <- tmEval Core.hnf Θ ;; tmPrint (Σi Θ)). *)
+
+(* Definition bar := Type. *)
+
+(* Run TemplateProgram (Translate ε "bar"). *)
+(* Print barᵗ. *)
+
+(* Definition foo (A : Type) (x : A) := x. *)
+
+(* Run TemplateProgram (Translate ε "foo"). *)
+(* Print fooᵗ. *)
+
+(* Definition pseudoid (A B : Type) (e : A = B) (x : A) : B := {! x !}. *)
+
+(* Run TemplateProgram (Translate ε "pseudoid"). *)
+(* Print pseudoidᵗ. *)
+
+(* Definition test (A B C : Type) (f : A -> B) (e : B = C) (u : B = A) (x : B) : C := *)
+(*   {! f {! x !} !}. *)
+
+(* Run TemplateProgram (Translate ε "test"). *)
+(* Print testᵗ. *)
+
+(* (* Definition AAmap (x :AA) := x. *) *)
+(* Definition AA' := AA. *)
+(* Fail Run TemplateProgram (Translate ε "AA'"). *)
+(* Run TemplateProgram (Θ <- TranslateConstant ε "AA" ;; Translate Θ "AA'"). *)
+(* Print AA'ᵗ. *)
+
+(* Definition zero := 0. *)
+(* Fail Run TemplateProgram (Translate ε "zero"). *)
+(* Run TemplateProgram (Θ <- TranslateConstant ε "nat" ;; Translate Θ "zero"). *)
+(* Print zeroᵗ. *)
+
+(* Definition nat' := nat. *)
+(* Fail Run TemplateProgram (Translate ε "nat'"). *)
+(* Run TemplateProgram (Θ <- TranslateConstant ε "nat" ;; Translate Θ "nat'"). *)
+(* Print nat'ᵗ. *)
+
+Definition vrev {A n m} (v : vec A n) (acc : vec A m) : vec A (n + m) :=
+  vec_rect A (fun n _ => forall m, vec A m -> vec A (n + m))
+           (fun m acc => acc) (fun a n _ rv m acc => {! rv _ (vcons a m acc) !})
+           n v m acc.
+
+Run TemplateProgram (
+      Θ <- TranslateConstant ε "nat" ;;
+      Θ <- TranslateConstant Θ "vec" ;;
+      Θ <- TranslateConstant Θ "Nat.add" ;;
+      Θ <- TranslateConstant Θ "vec_rect" ;;
+      Translate Θ "vrev"
+      (* tmPrint Θ *)
+).
